examples/iso_dh/DY.Example.DH.Protocol.Total.Proof.fst
@@ -12,6 +12,8 @@ open DY.Example.DH.Protocol.Stateful
 
 val dh_crypto_usages: crypto_usages
 instance dh_crypto_usages = {
+  default_crypto_usages with
+
   dh_known_peer_usage = (fun s1 s2 ->
     match s1, s2 with
     | "DH.dh_key", _ -> AeadKey "DH.aead_key"
@@ -24,14 +26,6 @@ instance dh_crypto_usages = {
     | _ -> NoUsage);
   dh_known_peer_usage_commutes = (fun s1 s2 -> ());
   dh_unknown_peer_usage_implies = (fun s1 s2 -> ());
-
-  kdf_extract_usage = (fun salt_usg ikm_usg salt ikm -> NoUsage);
-  kdf_extract_label = (fun salt_usg ikm_usg salt_label ikm_label salt ikm -> salt_label `meet` ikm_label);
-  kdf_extract_label_lemma = (fun tr salt_usg ikm_usg salt_label ikm_label salt ikm -> ());
-
-  kdf_expand_usage = (fun prk_usage info -> NoUsage);
-  kdf_expand_label = (fun prk_usage prk_label info -> prk_label);
-  kdf_expand_label_lemma = (fun tr prk_usage prk_label info -> ());
 }
 
 #push-options "--ifuel 2 --fuel 0"
@@ -44,10 +38,10 @@ let dh_crypto_preds = {
     (exists prin. get_signkey_label vk = principal_label prin /\ (
       match parse sig_message sig_msg with
       | Some (SigMsg2 sig_msg2) -> (
-        exists y. sig_msg2.gy == (dh_pk y) /\ event_triggered tr prin (Respond1 sig_msg2.a prin sig_msg2.gx sig_msg2.gy y)
+        exists y. sig_msg2.gy == (dh_pk y) /\ event_triggered tr prin (Respond1 sig_msg2.alice prin sig_msg2.gx sig_msg2.gy y)
       )
       | Some (SigMsg3 sig_msg3) -> (
-        exists x k. sig_msg3.gx == (dh_pk x) /\ event_triggered tr prin (Initiate2 prin sig_msg3.b sig_msg3.gx sig_msg3.gy k)
+        exists x k. sig_msg3.gx == (dh_pk x) /\ event_triggered tr prin (Initiate2 prin sig_msg3.bob sig_msg3.gx sig_msg3.gy k)
       )
       | None -> False
     ))
@@ -73,22 +67,19 @@ val compute_message1_proof:
       DhKey? (get_usage x)
     )
     (ensures 
-      is_publishable tr (compute_message1 alice x) /\
-      (exists gx. gx == dh_pk x /\ is_publishable tr gx)
+      is_publishable tr (compute_message1 alice x)
     )
 let compute_message1_proof tr alice bob x si =
   let gx = dh_pk x in
   assert(is_publishable tr gx);
   let msg = Msg1 {alice; gx} in
 
-  // This lemma makes sure that the second argument
-  // (is_publishable tr) is true for the third argument
-  // (msg) before and after serialization. Without
-  // this lemma we would loose all the guarantees about
-  // the bytes after the message was serialized.
+  // This lemma
+  // - requires that msg.gx is is publishable
+  // - ensures that `serialize _ msg` is publishable
   serialize_wf_lemma message (is_publishable tr) msg;
 
-  // The following code is not needed for the prove.
+  // The following code is not needed for the proof.
   // It just shows what we need to show to prove the lemma.
   let msgb = compute_message1 alice x in 
   assert(bytes_invariant tr msgb);
@@ -112,15 +103,14 @@ val decode_message1_proof:
 let decode_message1_proof tr alice bob msg_bytes =
   match decode_message1 msg_bytes with
     | Some msg1 -> (
-      // The second argument of the lemma parse_wf_lemma is a predicate defined
-      // on bytes (is_publishable tr).
-      // The lemma has the precondition that the predicate is true if the
-      // third argument is applied to the predicate.
-      // It then makes sure that the predicate is also true after
-      // parsing the third argument from bytes into a data type (message).
+      // This lemma
+      // - requires that msg_bytes is publishable
+      // - ensures that `msg1.gx` is publishable
+      //   (`msg1` being the result of parsing `msg_bytes` to the type `message1`)
       parse_wf_lemma message (is_publishable tr) msg_bytes;
       
-      // Only for debugging purposes
+      // The following code is not needed for the proof.
+      // It just shows what we need to show to prove the lemma.
       assert(bytes_invariant tr msg1.gx);
       assert(get_label msg1.gx `can_flow tr` public);
       ()
@@ -130,11 +120,11 @@ let decode_message1_proof tr alice bob msg_bytes =
 val compute_message2_proof:
   tr:trace -> si:state_id ->
   alice:principal -> bob:principal ->
-  msg1:message1 ->
-  gy:bytes -> y:bytes ->
+  msg1:message1 -> y:bytes ->
   sk_b:bytes -> n_sig:bytes ->
   Lemma
-  (requires
+  (requires (
+    let gy = dh_pk y in
     event_triggered tr bob (Respond1 alice bob msg1.gx gy y) /\
     is_publishable tr msg1.gx /\ is_publishable tr gy /\
     gy == dh_pk y /\
@@ -142,49 +132,39 @@ val compute_message2_proof:
     is_signature_key "DH.SigningKey" (principal_label bob) tr sk_b /\
     is_secret (principal_label bob) tr n_sig /\
     SigNonce? (get_usage n_sig)
+    )
   )
-  (ensures
+  (ensures (
+    let gy = dh_pk y in
     is_publishable tr (compute_message2 alice bob msg1.gx gy sk_b n_sig)
+    )
   )
-let compute_message2_proof tr si alice bob msg1 gy y sk_b n_sig =
-  let sig_msg = SigMsg2 {a=alice; gx=msg1.gx; gy} in
+let compute_message2_proof tr si alice bob msg1 y sk_b n_sig =
+  // Proof that the SigMsg2 is publishable
+  // From the precondition we know that
+  // msg1.gx and gy are publishable.
+  let gy = dh_pk y in
+  let sig_msg = SigMsg2 {alice; gx=msg1.gx; gy} in
   serialize_wf_lemma sig_message (is_publishable tr) sig_msg;
   let sig_msg_bytes = serialize sig_message sig_msg in
-  //assert(is_publishable tr sig_msg_bytes);
+
+  // This assert is not needed for the proof
+  // but shows that the serialized SigMsg2 is publishable.
+  assert(is_publishable tr sig_msg_bytes);
+
   let sg = sign sk_b n_sig sig_msg_bytes in
-  
-  (*assert(bytes_invariant tr sk_b);
-  assert(bytes_invariant tr n_sig);
-  assert(bytes_invariant tr sig_msg_bytes);
-  assert(get_usage sk_b == SigKey "DH.SigningKey");
-  assert(is_secret (principal_label bob) tr sk_b);
-  assert(SigKey? (get_usage sk_b));*)
-  
-  // The reveal_opaques is needed to look into the definition
-  // of get_signkey_usage and see that it simply calls
-  // get_usage on the given key.
-  //reveal_opaque (`%get_signkey_usage) (get_signkey_usage);
-  
-  (*assert(SigKey? (get_signkey_usage (Vk sk_b)));
-  assert(get_signkey_usage (Vk sk_b) == SigKey "DH.SigningKey");
-  assert((SigMsg2?.msg sig_msg).gy == (dh_pk y));*)
 
-  //reveal_opaque (`%get_signkey_label) (get_signkey_label);
-  (*assert(exists prin. get_signkey_label (Vk sk_b) = principal_label prin /\
-    (SigMsg2?.msg sig_msg).gy == (dh_pk y) /\ 
-    event_triggered tr prin (Respond1 (SigMsg2?.msg sig_msg).a prin (SigMsg2?.msg sig_msg).gx (SigMsg2?.msg sig_msg).gy y));
-  assert(dh_crypto_invs.preds.sign_pred tr (Vk sk_b) sig_msg_bytes) by (let open FStar.Tactics in dump "");
-  assert(SigNonce? (get_usage n_sig));
-  assert((get_label sig_msg_bytes) `can_flow tr` (get_label n_sig));
+  // This assert is not needed for the proof
+  // but shows that the signature is also publishable.
+  assert(is_publishable tr sg);
   
-  assert(bytes_invariant tr sg);
-
-  assert(is_publishable tr sg);*)
+  // Since all parts of the Msg2 are publishable, we
+  // can show that the serialized Msg2 is also publishable.
   let msg = Msg2 {bob; gy; sg} in
   serialize_wf_lemma message (is_publishable tr) msg;
 
-  //let msg_bytes = compute_message2 alice bob msg1.gx gy sk_b n_sig in
-  //assert(bytes_invariant tr msg_bytes);
+  // This proves the post-condition
+  assert(is_publishable tr (compute_message2 alice bob msg1.gx gy sk_b n_sig));
   ()
 
 val decode_message2_proof:
@@ -200,10 +180,9 @@ val decode_message2_proof:
   (ensures (
     match decode_message2 msg_bytes alice gx pk_b with
     | Some msg2 -> (
-      let sig_msg = SigMsg2 {a=alice; gx; gy=msg2.gy} in
+      let sig_msg = SigMsg2 {alice; gx; gy=msg2.gy} in
       is_publishable tr msg2.gy /\
       is_publishable tr msg2.sg /\
-      verify pk_b (serialize sig_message sig_msg) msg2.sg /\
       (is_corrupt tr (principal_label alice) \/ is_corrupt tr (principal_label bob) \/
       (exists y. event_triggered tr bob (Respond1 alice bob gx msg2.gy y)))
     )
@@ -213,50 +192,17 @@ let decode_message2_proof tr alice bob msg_bytes gx pk_b =
   match decode_message2 msg_bytes alice gx pk_b with
     | Some msg2 -> (
       parse_wf_lemma message (is_publishable tr) msg_bytes;
-      //FStar.Classical.move_requires (parse_wf_lemma message (bytes_invariant tr)) msg_bytes;
+      serialize_wf_lemma sig_message (bytes_invariant tr) (SigMsg2 {alice; gx; gy = msg2.gy});
 
-      serialize_wf_lemma sig_message (bytes_invariant tr) (SigMsg2 {a=alice; gx; gy = msg2.gy});
-      
-      //reveal_opaque (`%verify) (verify);
-
-      // Revealing a recursive function does not work with
-      // ``reveal_opaque``. That's why we need to use
-      // ``normalize_term_spec bytes_invariant;`` or 
-      // ``norm_spec [zeta; delta_only [`%bytes_invariant]](bytes_invariant);``
-      //normalize_term_spec bytes_invariant;
-
-      (*assert(bytes_invariant tr msg_bytes);      
-      assert(bytes_invariant tr msg2.sg);
-
-      let sig_msg = SigMsg2 {a=alice; gx; gy=msg2.gy} in
-      
-      let sig_msg_bytes = serialize sig_message sig_msg in
-      assert(verify pk_b sig_msg_bytes msg2.sg = true);
-      
-      let open DY.Core.Bytes.Type in
-      let Sign sk nonce msg = msg2.sg in
-      assert(msg = sig_msg_bytes);
-      
+      // The following code is not needed for the proof.
+      // It just shows what we need to show to prove the lemma.
       assert(is_publishable tr msg2.sg);
-      assert(get_label msg2.sg `can_flow tr` get_label msg);
-      assert(get_label msg2.sg `can_flow tr` public);
-      
-      
-      normalize_term_spec get_label;
-
-      assert(bytes_invariant tr msg);
-      assert(is_publishable tr msg);
-      
-      FStar.Classical.move_requires (parse_wf_lemma sig_message (is_publishable tr)) msg;
-      FStar.Classical.move_requires (parse_wf_lemma sig_message (bytes_invariant tr)) msg;
-
-      assert(bytes_invariant tr gx);
-      assert(bytes_invariant tr msg2.gy);
+      assert(is_publishable tr msg2.gy);
       
       assert(is_corrupt tr (principal_label alice) \/
         is_corrupt tr (principal_label bob) \/
         (exists y. msg2.gy == dh_pk y /\ event_triggered tr bob (Respond1 alice bob gx msg2.gy y))
-      );*)
+      );
       ()
     )
     | None -> ()
@@ -278,23 +224,26 @@ val compute_message3_proof:
     is_publishable tr (compute_message3 alice bob gx gy sk_a n_sig)
   )
 let compute_message3_proof tr alice bob gx gy sk_a n_sig =
-  let sig_msg = SigMsg3 {b=bob; gx; gy} in
+  let sig_msg = SigMsg3 {bob; gx; gy} in
   serialize_wf_lemma sig_message (is_publishable tr) sig_msg;
   
-  (* Debugging code
-  assert(is_publishable tr (serialize sig_message sig_msg));*)
+  // The following code is not needed for the proof.
+  // It just shows what we need to show to prove the lemma.
+  assert(is_publishable tr (serialize sig_message sig_msg));
   let sg = sign sk_a n_sig (serialize sig_message sig_msg) in 
 
-  (* Debugging code 
+  // The following code is not needed for the proof.
+  // It just shows what we need to show to prove the lemma. 
   assert(get_label sg `can_flow tr` public);
   assert(bytes_invariant tr sg);
-  assert(is_publishable tr sg); *)
+  assert(is_publishable tr sg);
 
   let msg = Msg3 {sg} in
   serialize_wf_lemma message (is_publishable tr) msg;
 
-  (* Debugging code
-  assert(is_publishable tr (serialize message msg));*)
+  // The following code is not needed for the proof.
+  // It just shows what we need to show to prove the lemma.
+  assert(is_publishable tr (serialize message msg));
   ()
 
 val decode_message3_proof:
@@ -310,9 +259,8 @@ val decode_message3_proof:
   (ensures (
     match decode_message3 msg_bytes bob gx gy pk_a with
     | Some msg3 -> (
-      let sig_msg = SigMsg3 {b=bob; gx; gy} in
+      let sig_msg = SigMsg3 {bob; gx; gy} in
       is_publishable tr msg3.sg /\
-      verify pk_a (serialize sig_message sig_msg) msg3.sg /\
       (is_corrupt tr (principal_label alice) \/
       (exists x k. gx == dh_pk x /\ event_triggered tr alice (Initiate2 alice bob gx gy k)))
     )
@@ -322,7 +270,7 @@ let decode_message3_proof tr alice bob gx gy msg_bytes pk_a =
   match decode_message3 msg_bytes bob gx gy pk_a with
     | Some msg3 -> (
       parse_wf_lemma message (is_publishable tr) msg_bytes;
-      serialize_wf_lemma sig_message (is_publishable tr) (SigMsg3 {b=bob; gx; gy});
+      serialize_wf_lemma sig_message (is_publishable tr) (SigMsg3 {bob; gx; gy});
       ()
     )
     | None -> ()
